- Finished proofs supporting the cap_encode_decode lemma - Multiple new auxiliary lemmas on conversions to/from bits/bools and on try_maps - Generalized bv_to_bits_to_Z and mword_of_bits_to_mword_of_bools to any bv length - Simplified bool_bits_of_bytes

theories/Common/Utils.v
@@ -75,7 +75,7 @@ Definition bool_bits_of_bytes (bytes : list ascii): list bool
     | Ascii a0 a1 a2 a3 a4 a5 a6 a7 => [a7; a6; a5; a4; a3; a2; a1; a0]
     end
   in
-  List.fold_left (fun l a => List.app l (ascii_to_bits a)) bytes [].
+  List.concat (map ascii_to_bits bytes).
 
 (* could be generalized as monadic map, or implemented as composition
    of [map] and [sequence]. *)
